DPE: bring functional correctness props up from Engine/L0 into DPE context.

pulse/share/steel/examples/pulse/dice/dpe/DPE.fst
@@ -9,7 +9,7 @@ open L0Core
 module L = Pulse.Lib.SpinLock
 module A = Pulse.Lib.Array
 module R = Pulse.Lib.Reference
-module US = FStar.SizeT
+module SZ = FStar.SizeT
 module U8 = FStar.UInt8
 module U32 = FStar.UInt32
 module HT = Pulse.Lib.HashTable
@@ -21,77 +21,177 @@ val run_stt (#a:Type) (#post:a -> vprop) (f:stt a emp post) : a
 
 (* Engine Context *)
 noeq
-type engine_context = { uds: A.larray U8.t (US.v uds_len); }
+type engine_context_t = { 
+  uds: A.larray U8.t (US.v uds_len); 
+}
 
-let engine_context_perm (c:engine_context) : vprop
+let engine_context_perm (c:engine_context_t) : vprop
   = A.pts_to c.uds full_perm uds_bytes ** 
     pure (A.is_full_array c.uds)
 
-let mk_engine_context uds : engine_context = {uds}
+let mk_engine_context_t uds : engine_context_t = {uds}
 
 (* L0 Context *)
 noeq
-type l0_context = { cdi: A.larray U8.t (US.v dice_digest_len); }
+type l0_context_t = { 
+  cdi:A.larray U8.t (US.v dice_digest_len); 
+}
 
-// FIXME: lost cdi_functional_correctness! 
-let l0_context_perm (c:l0_context) : vprop
-  = exists_ (fun (s:elseq U8.t dice_digest_len) -> A.pts_to c.cdi full_perm s) **
-    pure (A.is_full_array c.cdi)
+let mk_l0_context_t cdi : l0_context_t = {cdi}
 
-let mk_l0_context cdi : l0_context = {cdi}
+type l0_context_repr_t = {
+  cdi:elseq U8.t dice_digest_len;
+  repr:engine_record_repr;
+}
+
+let mk_l0_context_repr_t
+  (cdi:erased (elseq U8.t dice_digest_len)) 
+  (repr:erased engine_record_repr) 
+: erased l0_context_repr_t 
+= {cdi; repr}
+
+let l0_context_perm (c:l0_context_t) (r:l0_context_repr_t): vprop
+  = A.pts_to c.cdi full_perm r.cdi **
+    pure (A.is_full_array c.cdi
+       /\ cdi_functional_correctness r.cdi r.repr
+       /\ l0_is_authentic r.repr)
+
 
 (* L1 Context *)
 noeq
-type l1_context = { deviceID_priv: A.larray U8.t (US.v v32us);
-                    deviceID_pub: A.larray U8.t (US.v v32us);
+type l1_context_t = { deviceID_priv: A.larray U8.t (US.v v32us);
+                    deviceID_pub: A.larray U8.t (US.v v32us);   
                     aliasKey_priv: A.larray U8.t (US.v v32us);
                     aliasKey_pub: A.larray U8.t (US.v v32us);
                     aliasKeyCRT: A.array U8.t;
                     deviceIDCSR: A.array U8.t; }
 
-// FIXME: lost functoinal correctness! 
-let l1_context_perm (c:l1_context)
+let mk_l1_context_t deviceID_priv deviceID_pub aliasKey_priv aliasKey_pub aliasKeyCRT deviceIDCSR 
+: l1_context_t
+= { deviceID_priv; deviceID_pub; aliasKey_priv; aliasKey_pub; aliasKeyCRT; deviceIDCSR }
+
+noeq
+type l1_context_repr_t = {
+  deviceID_label_len: hkdf_lbl_len;
+  aliasKey_label_len: hkdf_lbl_len;
+  deviceID_priv: elseq U8.t v32us;
+  deviceID_pub: elseq U8.t v32us;
+  aliasKey_priv: elseq U8.t v32us;
+  aliasKey_pub:elseq U8.t v32us;
+  aliasKeyCRT_len:SZ.t;
+  aliasKeyCRT: elseq U8.t aliasKeyCRT_len;
+  deviceIDCSR_len:SZ.t;
+  deviceIDCSR:elseq U8.t deviceIDCSR_len;
+  cdi:elseq U8.t dice_digest_len;
+  repr:l0_record_repr;
+  deviceIDCSR_ingredients: deviceIDCSR_ingredients_t;
+  aliasKeyCRT_ingredients: aliasKeyCRT_ingredients_t;
+}
+
+let mk_l1_context_repr_t 
+  (deviceID_label_len:erased hkdf_lbl_len)
+  (aliasKey_label_len:erased hkdf_lbl_len)
+  (deviceID_priv:erased (elseq U8.t v32us))
+  (deviceID_pub:erased (elseq U8.t v32us))
+  (aliasKey_priv:erased (elseq U8.t v32us))
+  (aliasKey_pub:erased (elseq U8.t v32us))
+  (aliasKeyCRT_len:erased SZ.t)
+  (aliasKeyCRT:erased (elseq U8.t aliasKeyCRT_len))
+  (deviceIDCSR_len:erased SZ.t)
+  (deviceIDCSR:erased (elseq U8.t deviceIDCSR_len))
+  (cdi:erased (elseq U8.t dice_digest_len))
+  (repr:erased l0_record_repr)
+  (deviceIDCSR_ingredients:erased deviceIDCSR_ingredients_t)
+  (aliasKeyCRT_ingredients:erased aliasKeyCRT_ingredients_t)
+: erased l1_context_repr_t 
+= {deviceID_label_len; aliasKey_label_len; deviceID_priv; deviceID_pub; aliasKey_priv;
+  aliasKey_pub; aliasKeyCRT_len; aliasKeyCRT; deviceIDCSR_len; deviceIDCSR;
+  cdi; repr; deviceIDCSR_ingredients; aliasKeyCRT_ingredients}
+
+let l1_context_perm (c:l1_context_t) (r:l1_context_repr_t)
   : vprop
-  = exists_ (fun s -> A.pts_to c.deviceID_priv full_perm s) **
-    exists_ (fun s -> A.pts_to c.deviceID_pub full_perm s) **
-    exists_ (fun s -> A.pts_to c.aliasKey_priv full_perm s) **
-    exists_ (fun s -> A.pts_to c.aliasKey_pub full_perm s) **
-    exists_ (fun s -> A.pts_to c.aliasKeyCRT full_perm s) **
-    exists_ (fun s -> A.pts_to c.deviceIDCSR full_perm s) **
+  = A.pts_to c.deviceID_priv full_perm r.deviceID_priv **
+    A.pts_to c.deviceID_pub full_perm r.deviceID_pub **
+    A.pts_to c.aliasKey_priv full_perm r.aliasKey_priv **
+    A.pts_to c.aliasKey_pub full_perm r.aliasKey_pub **
+    A.pts_to c.aliasKeyCRT full_perm r.aliasKeyCRT **
+    A.pts_to c.deviceIDCSR full_perm r.deviceIDCSR **
     pure (
+      valid_hkdf_ikm_len dice_digest_len /\
+      aliasKey_functional_correctness
+        dice_hash_alg dice_digest_len r.cdi r.repr.fwid
+        r.aliasKey_label_len r.repr.aliasKey_label 
+        r.aliasKey_pub r.aliasKey_priv /\
+      deviceIDCSR_functional_correctness 
+        dice_hash_alg dice_digest_len r.cdi
+        r.deviceID_label_len r.repr.deviceID_label r.deviceIDCSR_ingredients 
+        r.deviceIDCSR_len r.deviceIDCSR /\       
+      aliasKeyCRT_functional_correctness 
+        dice_hash_alg dice_digest_len r.cdi r.repr.fwid
+        r.deviceID_label_len r.repr.deviceID_label r.aliasKeyCRT_ingredients 
+        r.aliasKeyCRT_len r.aliasKeyCRT r.aliasKey_pub /\
       A.is_full_array c.deviceID_priv /\
       A.is_full_array c.deviceID_pub /\
       A.is_full_array c.aliasKey_priv /\
       A.is_full_array c.aliasKey_pub /\
       A.is_full_array c.aliasKeyCRT /\
       A.is_full_array c.deviceIDCSR
-    )
-
-let mk_l1_context deviceID_priv deviceID_pub aliasKey_priv aliasKey_pub aliasKeyCRT deviceIDCSR 
-  = { deviceID_priv; deviceID_pub; aliasKey_priv; aliasKey_pub; aliasKeyCRT; deviceIDCSR }
-  
+    )  
 
 (* Generic Context *)    // this is called an enumeration
 noeq
 type context_t = 
-  | Engine_context : c:engine_context -> context_t
-  | L0_context     : c:l0_context -> context_t
-  | L1_context     : c:l1_context -> context_t
+  | Engine_context : c:engine_context_t -> context_t
+  | L0_context     : c:l0_context_t -> context_t
+  | L1_context     : c:l1_context_t -> context_t
 
-let context_perm (t:context_t) : vprop = 
-  match t with
+let mk_context_t_engine c = Engine_context c
+let mk_context_t_l0 c = L0_context c
+let mk_context_t_l1 c = L1_context c
+
+noeq
+type context_repr_t = 
+  | Engine_context_repr : context_repr_t
+  | L0_context_repr     : r:l0_context_repr_t -> context_repr_t
+  | L1_context_repr     : r:l1_context_repr_t -> context_repr_t
+
+let mk_context_repr_t_l0 (r:erased l0_context_repr_t) 
+: erased context_repr_t = L0_context_repr r
+let mk_context_repr_t_l1 (r:erased l1_context_repr_t) 
+: erased context_repr_t = L1_context_repr r
+
+let context_perm (context:context_t) (repr:context_repr_t): vprop = 
+  match context with
   | Engine_context c -> engine_context_perm c
-  | L0_context c -> l0_context_perm c
-  | L1_context c -> l1_context_perm c
+  | L0_context c -> (
+    match repr with 
+    | L0_context_repr r -> l0_context_perm c r
+    | _ -> pure(false)
+  )
+  | L1_context c -> (
+    match repr with
+    | L1_context_repr r -> l1_context_perm c r
+    | _ -> pure(false)
+  )
+
+assume val get_l0_context_perm (context:context_t{L0_context? context}) (repr:erased context_repr_t)
+  : stt_ghost (erased l0_context_repr_t) emp_inames
+              (context_perm context repr)
+              (fun r -> l0_context_perm (L0_context?.c context) r
+                      ** pure(reveal repr == L0_context_repr r))
+
+assume val get_l1_context_perm (context:context_t{L1_context? context}) (repr:erased context_repr_t)
+  : stt_ghost (erased l1_context_repr_t) emp_inames
+              (context_perm context repr)
+              (fun r -> l1_context_perm (L1_context?.c context) r
+                      ** pure(reveal repr == L1_context_repr r))
 
 // In the implmentation, we store contexts as values in a global hash table
 // so we need a way to store and retrieve permission on the context. We do this
 // by keeping a tuple of the context along with a lock on the context permission
-let locked_context_t = c:context_t & L.lock (context_perm c)
-
-let mk_engine_context_t engine_context = Engine_context engine_context
-let mk_l0_context_t l0_context = L0_context l0_context
-let mk_l1_context_t l1_context = L1_context l1_context
+let locked_context_t = c:context_t 
+                     & r:erased context_repr_t 
+                     & L.lock (context_perm c r)
 
 (* Record *)
 noeq
@@ -122,19 +222,7 @@ assume val get_engine_record_perm (record:record_t{Engine_record? record}) (repr
               (record_perm record repr)
               (fun r0 -> engine_record_perm (Engine_record?.r record) r0 
                       ** pure(reveal repr == Engine_repr r0))
-// ```pulse
-// ghost fn get_engine_record_perm (record:(r:record_t{Engine_record? r})) (repr:erased repr_t)
-//   requires record_perm record repr
-//   returns r0:erased engine_record_repr
-//   ensures engine_record_perm (Engine_record?.r record) r0 ** pure(repr == Engine_repr r0)
-// {
-//   let r = Engine_record?.r record;
-//   match (reveal repr) { 
-//   Engine_repr r0 -> {admit()}
-//   _ -> {admit()}
-//   }
-// }
-// ```
+
 assume val get_l0_record_perm (record:record_t{L0_record? record}) (repr:erased repr_t)
   : stt_ghost (erased l0_record_repr) emp_inames
               (record_perm record repr)
@@ -208,38 +296,48 @@ fn open_session' (_:unit)
 {
   let cht = alloc_ht #cht_sig cht_len;
 
-  let sht_lk = dsnd locked_sht;
-  let sid_lk = dsnd locked_sid;
+  let sht_lk = locked_sht._2;
+  let sid_lk = locked_sid._2;
 
-  L.acquire #(exists_ (fun n -> R.pts_to (dfst locked_sid) full_perm n)) sid_lk;
-  L.acquire #(exists_ (fun pht -> models sht_sig (dfst locked_sht) pht)) sht_lk;
+  L.acquire #(exists_ (fun n -> R.pts_to locked_sid._1 full_perm n)) sid_lk;
+  L.acquire #(exists_ (fun pht -> models sht_sig locked_sht._1 pht)) sht_lk;
 
-  let sid = !(dfst locked_sid);
+  let sid = !locked_sid._1;
 
-  with pht. assert (models sht_sig (dfst locked_sht) pht);
+  with pht. assert (models sht_sig locked_sht._1 pht);
 
-  let b = not_full #sht_sig #pht (dfst locked_sht);
+  let b = not_full #sht_sig #pht locked_sht._1;
 
   if b {
-    let r = HT.insert #sht_sig #pht (dfst locked_sht) sid cht;
-    with pht'. unfold (maybe_update r sht_sig (dfst locked_sht) pht pht');
+    let r = HT.insert #sht_sig #pht locked_sht._1 sid cht;
+    with pht'. unfold (maybe_update r sht_sig locked_sht._1 pht pht');
     if r {
-      assert (HT.models sht_sig (dfst locked_sht) (PHT.insert pht sid cht));
-      // dfst locked_sid := sid + 1ul; // FIXME: check whether sum fits into a U32
-      L.release #(exists_ (fun n -> R.pts_to (dfst locked_sid) full_perm n)) sid_lk;
-      L.release #(exists_ (fun pht -> models sht_sig (dfst locked_sht) pht)) sht_lk;
-      Some sid
+      assert (HT.models sht_sig locked_sht._1 (PHT.insert pht sid cht));
+      let opt_inc = sid `safe_add` 1ul;
+      match opt_inc {
+      Some inc -> {
+        locked_sid._1 := inc;
+        L.release #(exists_ (fun n -> R.pts_to locked_sid._1 full_perm n)) sid_lk;
+        L.release #(exists_ (fun pht -> models sht_sig locked_sht._1 pht)) sht_lk;
+        Some sid
+      }
+      None -> {
+        // ERROR - increment session ID failed
+        L.release #(exists_ (fun n -> R.pts_to locked_sid._1 full_perm n)) sid_lk;
+        L.release #(exists_ (fun pht -> models sht_sig locked_sht._1 pht)) sht_lk;
+        None #sid_t
+      }}
     } else {
       // ERROR - insert failed
-      assert (HT.models sht_sig (dfst locked_sht) pht);
-      L.release #(exists_ (fun n -> R.pts_to (dfst locked_sid) full_perm n)) sid_lk;
-      L.release #(exists_ (fun pht -> models sht_sig (dfst locked_sht) pht)) sht_lk;
+      assert (HT.models sht_sig locked_sht._1 pht);
+      L.release #(exists_ (fun n -> R.pts_to locked_sid._1 full_perm n)) sid_lk;
+      L.release #(exists_ (fun pht -> models sht_sig locked_sht._1 pht)) sht_lk;
       None #sid_t
     }
   } else {
     // ERROR - table full
-    L.release #(exists_ (fun n -> R.pts_to (dfst locked_sid) full_perm n)) sid_lk;
-    L.release #(exists_ (fun pht -> models sht_sig (dfst locked_sht) pht)) sht_lk;
+    L.release #(exists_ (fun n -> R.pts_to locked_sid._1 full_perm n)) sid_lk;
+    L.release #(exists_ (fun pht -> models sht_sig locked_sht._1 pht)) sht_lk;
     None #sid_t
   }
 }
@@ -259,27 +357,31 @@ fn disable_uds (_:unit)
 ```
 
 ```pulse 
-fn destroy_ctxt (ctxt:context_t)
-  requires context_perm ctxt
+fn destroy_ctxt (ctxt:context_t) (#repr:erased context_repr_t)
+  requires context_perm ctxt repr
   ensures emp
 {
   match ctxt {
   Engine_context c -> {
-    rewrite (context_perm ctxt) as (engine_context_perm c);
+    rewrite (context_perm ctxt repr) as (engine_context_perm c);
     unfold (engine_context_perm c);
     A.zeroize uds_len c.uds;
     A.free c.uds;
   }
   L0_context c -> {
-    rewrite (context_perm ctxt) as (l0_context_perm c);
-    unfold (l0_context_perm c);
+    let r = get_l0_context_perm ctxt repr;
+    rewrite (l0_context_perm (L0_context?.c ctxt) r)
+      as (l0_context_perm c r);
+    unfold (l0_context_perm c r);
     with s. assert (A.pts_to c.cdi full_perm s);
     A.zeroize dice_digest_len c.cdi;
     A.free c.cdi;
   }
   L1_context c -> {
-    rewrite (context_perm ctxt) as (l1_context_perm c);
-    unfold (l1_context_perm c);
+    let r = get_l1_context_perm ctxt repr;
+    rewrite (l1_context_perm (L1_context?.c ctxt) r)
+      as (l1_context_perm c r);
+    unfold (l1_context_perm c r);
     A.free c.deviceID_priv;
     A.free c.deviceID_pub;
     A.free c.aliasKey_priv;
@@ -295,9 +397,10 @@ fn destroy_locked_ctxt (locked_ctxt:locked_context_t)
   requires emp
   ensures emp
 {
-  let ctxt = dfst locked_ctxt;
-  let ctxt_lk = dsnd locked_ctxt;
-  L.acquire #(context_perm ctxt) ctxt_lk;
+  let ctxt = locked_ctxt._1;
+  let repr = locked_ctxt._2;
+  let ctxt_lk = locked_ctxt._3;
+  L.acquire #(context_perm ctxt repr) ctxt_lk;
   destroy_ctxt ctxt;
 }
 ```
@@ -315,50 +418,50 @@ fn destroy_context' (sid:sid_t) (ctxt_hndl:ctxt_hndl_t)
   returns b:bool
   ensures emp
 {
-  let sht_lk = dsnd locked_sht;
-  L.acquire #(exists_ (fun pht -> models sht_sig (dfst locked_sht) pht)) sht_lk;
+  let sht_lk = locked_sht._2;
+  L.acquire #(exists_ (fun pht -> models sht_sig locked_sht._1 pht)) sht_lk;
 
-  with spht. assert (models sht_sig (dfst locked_sht) spht);
+  with spht. assert (models sht_sig locked_sht._1 spht);
 
-  let res = HT.lookup #sht_sig #spht (dfst locked_sht) sid;
+  let res = HT.lookup #sht_sig #spht locked_sht._1 sid;
   if (fst res) {
     let opt_locked_cht = snd res;
     match opt_locked_cht {
     Some locked_cht -> {
-      let cht_lk = dsnd locked_cht;
-      L.acquire #(exists_ (fun pht -> models cht_sig (dfst locked_cht) pht)) cht_lk;
-      with cpht0. assert (models cht_sig (dfst locked_cht) cpht0);
+      let cht_lk = locked_cht._2;
+      L.acquire #(exists_ (fun pht -> models cht_sig locked_cht._1 pht)) cht_lk;
+      with cpht0. assert (models cht_sig locked_cht._1 cpht0);
 
-      let res = HT.lookup #cht_sig #cpht0 (dfst locked_cht) ctxt_hndl;
+      let res = HT.lookup #cht_sig #cpht0 locked_cht._1 ctxt_hndl;
       if (fst res) {
         let opt_locked_ctxt = snd res;
         match opt_locked_ctxt {
         Some locked_ctxt -> {
           destroy_locked_ctxt locked_ctxt;
-          L.release #(exists_ (fun pht -> models cht_sig (dfst locked_cht) pht)) cht_lk;
-          L.release #(exists_ (fun pht -> models sht_sig (dfst locked_sht) pht)) sht_lk;
+          L.release #(exists_ (fun pht -> models cht_sig locked_cht._1 pht)) cht_lk;
+          L.release #(exists_ (fun pht -> models sht_sig locked_sht._1 pht)) sht_lk;
           true
         }
         None -> {
           // ERROR - bad context handle
-          L.release #(exists_ (fun pht -> models cht_sig (dfst locked_cht) pht)) cht_lk;
-          L.release #(exists_ (fun pht -> models sht_sig (dfst locked_sht) pht)) sht_lk;
+          L.release #(exists_ (fun pht -> models cht_sig locked_cht._1 pht)) cht_lk;
+          L.release #(exists_ (fun pht -> models sht_sig locked_sht._1 pht)) sht_lk;
           false
         }}
       } else {
         // ERROR - lookup failed
-        L.release #(exists_ (fun pht -> models cht_sig (dfst locked_cht) pht)) cht_lk;
-        L.release #(exists_ (fun pht -> models sht_sig (dfst locked_sht) pht)) sht_lk;
+        L.release #(exists_ (fun pht -> models cht_sig locked_cht._1 pht)) cht_lk;
+        L.release #(exists_ (fun pht -> models sht_sig locked_sht._1 pht)) sht_lk;
         false
       }}
     None -> {
       // ERROR - bad session ID
-      L.release #(exists_ (fun pht -> models sht_sig (dfst locked_sht) pht)) sht_lk;
+      L.release #(exists_ (fun pht -> models sht_sig locked_sht._1 pht)) sht_lk;
       false
     }}
   } else {
     // ERROR - lookup failed
-    L.release #(exists_ (fun pht -> models sht_sig (dfst locked_sht) pht)) sht_lk;
+    L.release #(exists_ (fun pht -> models sht_sig locked_sht._1 pht)) sht_lk;
     false
   }
 }
@@ -386,41 +489,41 @@ fn close_session' (sid:sid_t)
   returns b:bool
   ensures emp
 {
-  let sht_lk = dsnd locked_sht;
-  L.acquire #(exists_ (fun pht -> models sht_sig (dfst locked_sht) pht)) sht_lk;
+  let sht_lk = locked_sht._2;
+  L.acquire #(exists_ (fun pht -> models sht_sig locked_sht._1 pht)) sht_lk;
 
-  with pht. assert (models sht_sig (dfst locked_sht) pht);
+  with pht. assert (models sht_sig locked_sht._1 pht);
 
-  let res = HT.lookup #sht_sig #pht (dfst locked_sht) sid;
+  let res = HT.lookup #sht_sig #pht locked_sht._1 sid;
   if (fst res) {
     let opt_locked_cht = snd res;
     match opt_locked_cht {
     Some locked_cht -> { 
-      let cht_lk = dsnd locked_cht;
+      let cht_lk = locked_cht._2;
       // Note: We don't release this lock because we give up permission
       // on the cht when we deallocate it
-      L.acquire #(exists_ (fun pht -> models cht_sig (dfst locked_cht) pht)) cht_lk;
-      dealloc #cht_sig (dfst locked_cht) cht_len destroy_locked_ctxt ctxt_hndl_do_nothing;
-      let b = HT.delete #sht_sig #pht (dfst locked_sht) sid;
-      with pht'. unfold (maybe_update b sht_sig (dfst locked_sht) pht pht');
+      L.acquire #(exists_ (fun pht -> models cht_sig locked_cht._1 pht)) cht_lk;
+      dealloc #cht_sig locked_cht._1 cht_len destroy_locked_ctxt ctxt_hndl_do_nothing;
+      let b = HT.delete #sht_sig #pht locked_sht._1 sid;
+      with pht'. unfold (maybe_update b sht_sig locked_sht._1 pht pht');
       if b {
-        assert (models sht_sig (dfst locked_sht) (PHT.delete pht sid));
-        L.release #(exists_ (fun pht -> models sht_sig (dfst locked_sht) pht)) sht_lk;
+        assert (models sht_sig locked_sht._1 (PHT.delete pht sid));
+        L.release #(exists_ (fun pht -> models sht_sig locked_sht._1 pht)) sht_lk;
         b
       } else {
-        assert (models sht_sig (dfst locked_sht) pht);
-        L.release #(exists_ (fun pht -> models sht_sig (dfst locked_sht) pht)) sht_lk;
+        assert (models sht_sig locked_sht._1 pht);
+        L.release #(exists_ (fun pht -> models sht_sig locked_sht._1 pht)) sht_lk;
         b
       }
     }
     None -> {
       // ERROR - bad session ID
-      L.release #(exists_ (fun pht -> models sht_sig (dfst locked_sht) pht)) sht_lk;
+      L.release #(exists_ (fun pht -> models sht_sig locked_sht._1 pht)) sht_lk;
       false
     }}
   } else {
     // ERROR - lookup failed
-    L.release #(exists_ (fun pht -> models sht_sig (dfst locked_sht) pht)) sht_lk;
+    L.release #(exists_ (fun pht -> models sht_sig locked_sht._1 pht)) sht_lk;
     false
   }
 }
@@ -440,23 +543,27 @@ fn init_engine_ctxt (uds:A.larray U8.t (US.v uds_len)) (#p:perm)
   let uds_buf = A.alloc 0uy uds_len;
   memcpy uds_len uds uds_buf;
   disable_uds ();
-  let engine_context = mk_engine_context uds_buf;
+  let engine_context = mk_engine_context_t uds_buf;
 
   rewrite (A.pts_to uds_buf full_perm uds_bytes) 
     as (A.pts_to engine_context.uds full_perm uds_bytes);
   fold (engine_context_perm engine_context);
 
-  let ctxt = mk_engine_context_t engine_context;
+  let ctxt = mk_context_t_engine engine_context;
+  rewrite (engine_context_perm engine_context) 
+    as (context_perm ctxt Engine_context_repr);
 
-  rewrite (engine_context_perm engine_context) as (context_perm ctxt);
-
-  let ctxt_lk = L.new_lock (context_perm ctxt);
-  ((| ctxt, ctxt_lk |) <: locked_context_t)
+  let ctxt_lk = L.new_lock (context_perm ctxt Engine_context_repr);
+  ((| ctxt, hide Engine_context_repr, ctxt_lk |) <: locked_context_t)
 }
 ```
 
 ```pulse
-fn _init_l0_ctxt (cdi:A.larray U8.t (US.v dice_digest_len)) (#s:erased (elseq U8.t dice_digest_len))
+fn init_l0_ctxt (cdi:A.larray U8.t (US.v dice_digest_len)) 
+  (#engine_repr:erased engine_record_repr)
+  (#s:erased (elseq U8.t dice_digest_len))
+  (_:squash(cdi_functional_correctness s engine_repr
+         /\ l0_is_authentic engine_repr))
   requires A.pts_to cdi full_perm s
         ** pure (A.is_full_array cdi)
   returns _:locked_context_t
@@ -467,42 +574,62 @@ fn _init_l0_ctxt (cdi:A.larray U8.t (US.v dice_digest_len)) (#s:erased (elseq U8
   A.zeroize dice_digest_len cdi;
   A.free cdi;
 
-  let l0_context = mk_l0_context cdi_buf;
+  let l0_context = mk_l0_context_t cdi_buf;
+  let l0_context_repr = mk_l0_context_repr_t s engine_repr;
   rewrite (A.pts_to cdi_buf full_perm s)
     as (A.pts_to l0_context.cdi full_perm s);
-  fold (l0_context_perm l0_context);
-  let ctxt = mk_l0_context_t l0_context;
-  rewrite (l0_context_perm l0_context) as (context_perm ctxt);
-  let ctxt_lk = L.new_lock (context_perm ctxt);
-  ((| ctxt, ctxt_lk |) <: locked_context_t)
+  fold (l0_context_perm l0_context l0_context_repr);
+
+  let ctxt = mk_context_t_l0 l0_context;
+  let repr = mk_context_repr_t_l0 l0_context_repr;
+  rewrite (l0_context_perm l0_context l0_context_repr) 
+    as (context_perm ctxt repr);
+
+  let ctxt_lk = L.new_lock (context_perm ctxt repr);
+  ((| ctxt, repr, ctxt_lk |) <: locked_context_t)
 }
 ```
-let init_l0_ctxt cdi #s = _init_l0_ctxt cdi #s
-
-assume val coerce_seq_create (l:US.t) (s:(Seq.seq U8.t){s == Seq.create (US.v l) 0uy}) : elseq U8.t l
 
 ```pulse
-fn _init_l1_ctxt (deviceIDCSR_len: US.t) (aliasKeyCRT_len: US.t) 
+fn init_l1_ctxt (deviceIDCSR_len: US.t) (aliasKeyCRT_len: US.t) 
                 (deviceID_priv: A.larray U8.t (US.v v32us)) (deviceID_pub: A.larray U8.t (US.v v32us))
                 (aliasKey_priv: A.larray U8.t (US.v v32us)) (aliasKey_pub: A.larray U8.t (US.v v32us)) 
                 (deviceIDCSR: A.larray U8.t (US.v deviceIDCSR_len)) (aliasKeyCRT: A.larray U8.t (US.v aliasKeyCRT_len))
-                (#s1 #s2 #s3 #s4: erased (elseq U8.t v32us)) 
-                (#s5:erased (elseq U8.t deviceIDCSR_len))
-                (#s6:erased (elseq U8.t aliasKeyCRT_len))
-  requires A.pts_to deviceID_priv full_perm s1 ** 
-           A.pts_to deviceID_pub full_perm s2 ** 
-           A.pts_to aliasKey_priv full_perm s3 ** 
-           A.pts_to aliasKey_pub full_perm s4 ** 
-           A.pts_to deviceIDCSR full_perm s5 **
-           A.pts_to aliasKeyCRT full_perm s6
+                (#deviceID_priv0 #deviceID_pub0 #aliasKey_priv0 #aliasKey_pub0: erased (elseq U8.t v32us)) 
+                (#deviceIDCSR0:erased (elseq U8.t deviceIDCSR_len))
+                (#aliasKeyCRT0:erased (elseq U8.t aliasKeyCRT_len))
+                (#deviceID_label_len #aliasKey_label_len: erased hkdf_lbl_len)
+                (#cdi:erased (elseq U8.t dice_digest_len))
+                (#repr:erased l0_record_repr)
+                (#deviceIDCSR_ingredients:erased deviceIDCSR_ingredients_t)
+                (#aliasKeyCRT_ingredients:erased aliasKeyCRT_ingredients_t)
+                (_:squash(valid_hkdf_ikm_len dice_digest_len
+                       /\ aliasKey_functional_correctness
+                            dice_hash_alg dice_digest_len cdi repr.fwid
+                            aliasKey_label_len repr.aliasKey_label 
+                            aliasKey_pub0 aliasKey_priv0
+                       /\ deviceIDCSR_functional_correctness 
+                            dice_hash_alg dice_digest_len cdi
+                            deviceID_label_len repr.deviceID_label deviceIDCSR_ingredients 
+                            deviceIDCSR_len deviceIDCSR0 
+                       /\ aliasKeyCRT_functional_correctness 
+                            dice_hash_alg dice_digest_len cdi repr.fwid
+                            deviceID_label_len repr.deviceID_label aliasKeyCRT_ingredients 
+                            aliasKeyCRT_len aliasKeyCRT0 aliasKey_pub0))
+  requires A.pts_to deviceID_priv full_perm deviceID_priv0 ** 
+           A.pts_to deviceID_pub full_perm deviceID_pub0 ** 
+           A.pts_to aliasKey_priv full_perm aliasKey_priv0 ** 
+           A.pts_to aliasKey_pub full_perm aliasKey_pub0 ** 
+           A.pts_to deviceIDCSR full_perm deviceIDCSR0 **
+           A.pts_to aliasKeyCRT full_perm aliasKeyCRT0
   returns _:locked_context_t
   ensures 
-    A.pts_to deviceID_priv full_perm s1 ** 
-    A.pts_to deviceID_pub full_perm s2 **
-    A.pts_to aliasKey_priv full_perm s3 ** 
-    A.pts_to aliasKey_pub full_perm s4 ** 
-    A.pts_to deviceIDCSR full_perm s5 **
-    A.pts_to aliasKeyCRT full_perm s6
+    A.pts_to deviceID_priv full_perm deviceID_priv0 ** 
+    A.pts_to deviceID_pub full_perm deviceID_pub0 **
+    A.pts_to aliasKey_priv full_perm aliasKey_priv0 ** 
+    A.pts_to aliasKey_pub full_perm aliasKey_pub0 ** 
+    A.pts_to deviceIDCSR full_perm deviceIDCSR0 **
+    A.pts_to aliasKeyCRT full_perm aliasKeyCRT0
 {
   let deviceID_pub_buf = A.alloc 0uy v32us;
   let deviceID_priv_buf = A.alloc 0uy v32us;
@@ -517,30 +644,36 @@ fn _init_l1_ctxt (deviceIDCSR_len: US.t) (aliasKeyCRT_len: US.t)
   memcpy deviceIDCSR_len deviceIDCSR deviceIDCSR_buf;
   memcpy aliasKeyCRT_len aliasKeyCRT aliasKeyCRT_buf;
 
-  let l1_context = mk_l1_context deviceID_priv_buf deviceID_pub_buf aliasKey_priv_buf aliasKey_pub_buf aliasKeyCRT_buf deviceIDCSR_buf;
-  rewrite (A.pts_to deviceID_priv_buf full_perm s1 `star`
-           A.pts_to deviceID_pub_buf full_perm s2 `star`
-           A.pts_to aliasKey_priv_buf full_perm s3 `star`
-           A.pts_to aliasKey_pub_buf full_perm s4 `star`
-           A.pts_to deviceIDCSR_buf full_perm s5 `star`
-           A.pts_to aliasKeyCRT_buf full_perm s6)
-       as (A.pts_to l1_context.deviceID_priv full_perm s1`star`
-           A.pts_to l1_context.deviceID_pub full_perm s2 `star`
-           A.pts_to l1_context.aliasKey_priv full_perm s3 `star`
-           A.pts_to l1_context.aliasKey_pub full_perm s4 `star`
-           A.pts_to l1_context.deviceIDCSR full_perm s5 `star`
-           A.pts_to l1_context.aliasKeyCRT full_perm s6);
-  fold (l1_context_perm l1_context);
-  let ctxt = mk_l1_context_t l1_context;
-  rewrite (l1_context_perm l1_context) as (context_perm ctxt);
-  let ctxt_lk = L.new_lock (context_perm ctxt);
-  ((| ctxt, ctxt_lk |) <: locked_context_t)
+  let l1_context = mk_l1_context_t 
+    deviceID_priv_buf deviceID_pub_buf aliasKey_priv_buf aliasKey_pub_buf 
+    aliasKeyCRT_buf deviceIDCSR_buf;
+  let l1_context_repr = mk_l1_context_repr_t 
+    deviceID_label_len aliasKey_label_len deviceID_priv0 deviceID_pub0
+    aliasKey_priv0 aliasKey_pub0 aliasKeyCRT_len aliasKeyCRT0 deviceIDCSR_len
+    deviceIDCSR0 cdi repr deviceIDCSR_ingredients aliasKeyCRT_ingredients;
+
+  rewrite (A.pts_to deviceID_priv_buf full_perm deviceID_priv0 **
+           A.pts_to deviceID_pub_buf full_perm deviceID_pub0 **
+           A.pts_to aliasKey_priv_buf full_perm aliasKey_priv0 **
+           A.pts_to aliasKey_pub_buf full_perm aliasKey_pub0 **
+           A.pts_to deviceIDCSR_buf full_perm deviceIDCSR0 **
+           A.pts_to aliasKeyCRT_buf full_perm aliasKeyCRT0)
+       as (A.pts_to l1_context.deviceID_priv full_perm deviceID_priv0**
+           A.pts_to l1_context.deviceID_pub full_perm deviceID_pub0 **
+           A.pts_to l1_context.aliasKey_priv full_perm aliasKey_priv0 **
+           A.pts_to l1_context.aliasKey_pub full_perm aliasKey_pub0 **
+           A.pts_to l1_context.deviceIDCSR full_perm deviceIDCSR0 **
+           A.pts_to l1_context.aliasKeyCRT full_perm aliasKeyCRT0);
+  fold (l1_context_perm l1_context l1_context_repr);
+
+  let ctxt = mk_context_t_l1 l1_context;
+  let repr = mk_context_repr_t_l1 l1_context_repr;
+  rewrite (l1_context_perm l1_context l1_context_repr) as (context_perm ctxt repr);
+  
+  let ctxt_lk = L.new_lock (context_perm ctxt repr);
+  ((| ctxt, repr, ctxt_lk |) <: locked_context_t)
 }
 ```
-let init_l1_ctxt deviceIDCSR_len aliasKeyCRT_len deviceID_priv deviceID_pub
-  aliasKey_priv aliasKey_pub deviceIDCSR aliasKeyCRT #s1 #s2 #s3 #s4 #s5 #s6
-  = _init_l1_ctxt deviceIDCSR_len aliasKeyCRT_len deviceID_priv deviceID_pub
-    aliasKey_priv aliasKey_pub deviceIDCSR aliasKeyCRT #s1 #s2 #s3 #s4 #s5 #s6
 
 (*
   InitializeContext: Part of DPE API 
@@ -558,50 +691,50 @@ fn initialize_context' (sid:sid_t) (uds:A.larray U8.t (US.v uds_len)) (#p:perm)
   let locked_context = init_engine_ctxt uds;
   let ctxt_hndl = prng ();
 
-  let sht_lk = dsnd locked_sht;
-  L.acquire #(exists_ (fun pht -> models sht_sig (dfst locked_sht) pht)) sht_lk;
+  let sht_lk = locked_sht._2;
+  L.acquire #(exists_ (fun pht -> models sht_sig locked_sht._1 pht)) sht_lk;
 
-  with spht. assert (models sht_sig (dfst locked_sht) spht);
+  with spht. assert (models sht_sig locked_sht._1 spht);
 
-  let res = HT.lookup #sht_sig #spht (dfst locked_sht) sid;
+  let res = HT.lookup #sht_sig #spht locked_sht._1 sid;
   if (fst res) {
     let opt_locked_cht = snd res;
     match opt_locked_cht {
     Some locked_cht -> {
-      let cht_lk = dsnd locked_cht;
-      L.acquire #(exists_ (fun pht -> models cht_sig (dfst locked_cht) pht)) cht_lk;
+      let cht_lk = locked_cht._2;
+      L.acquire #(exists_ (fun pht -> models cht_sig locked_cht._1 pht)) cht_lk;
 
-      with cpht. assert (models cht_sig (dfst locked_cht) cpht);
-      let b = not_full #cht_sig #cpht (dfst locked_cht);
+      with cpht. assert (models cht_sig locked_cht._1 cpht);
+      let b = not_full #cht_sig #cpht locked_cht._1;
       if b {
-        let r = HT.insert #cht_sig #cpht (dfst locked_cht) ctxt_hndl locked_context;
-        with cpht'. unfold (maybe_update r cht_sig (dfst locked_cht) cpht cpht');
+        let r = HT.insert #cht_sig #cpht locked_cht._1 ctxt_hndl locked_context;
+        with cpht'. unfold (maybe_update r cht_sig locked_cht._1 cpht cpht');
         if r {
-          assert (models cht_sig (dfst locked_cht) (PHT.insert cpht ctxt_hndl locked_context));
-          L.release #(exists_ (fun pht -> models sht_sig (dfst locked_sht) pht)) sht_lk;
-          L.release #(exists_ (fun pht -> models cht_sig (dfst locked_cht) pht)) cht_lk;
+          assert (models cht_sig locked_cht._1 (PHT.insert cpht ctxt_hndl locked_context));
+          L.release #(exists_ (fun pht -> models sht_sig locked_sht._1 pht)) sht_lk;
+          L.release #(exists_ (fun pht -> models cht_sig locked_cht._1 pht)) cht_lk;
           Some ctxt_hndl
         } else {
           // ERROR - insert failed
-          assert (models cht_sig (dfst locked_cht) cpht);
-          L.release #(exists_ (fun pht -> models sht_sig (dfst locked_sht) pht)) sht_lk;
-          L.release #(exists_ (fun pht -> models cht_sig (dfst locked_cht) pht)) cht_lk;  
+          assert (models cht_sig locked_cht._1 cpht);
+          L.release #(exists_ (fun pht -> models sht_sig locked_sht._1 pht)) sht_lk;
+          L.release #(exists_ (fun pht -> models cht_sig locked_cht._1 pht)) cht_lk;  
           None #ctxt_hndl_t     
         }
       } else {
         // ERROR - table full
-        L.release #(exists_ (fun pht -> models sht_sig (dfst locked_sht) pht)) sht_lk;
-        L.release #(exists_ (fun pht -> models cht_sig (dfst locked_cht) pht)) cht_lk;
+        L.release #(exists_ (fun pht -> models sht_sig locked_sht._1 pht)) sht_lk;
+        L.release #(exists_ (fun pht -> models cht_sig locked_cht._1 pht)) cht_lk;
         None #ctxt_hndl_t
       }}
     None -> {
       // ERROR - bad session ID
-      L.release #(exists_ (fun pht -> models sht_sig (dfst locked_sht) pht)) sht_lk;
+      L.release #(exists_ (fun pht -> models sht_sig locked_sht._1 pht)) sht_lk;
       None #ctxt_hndl_t
     }}
   } else {
     // ERROR - lookup failed
-    L.release #(exists_ (fun pht -> models sht_sig (dfst locked_sht) pht)) sht_lk;
+    L.release #(exists_ (fun pht -> models sht_sig locked_sht._1 pht)) sht_lk;
     None #ctxt_hndl_t
   }
 }
@@ -621,75 +754,75 @@ fn rotate_context_handle' (sid:sid_t) (ctxt_hndl:ctxt_hndl_t)
 {
   let new_ctxt_hndl = prng ();
 
-  let sht_lk = dsnd locked_sht;
-  L.acquire #(exists_ (fun pht -> models sht_sig (dfst locked_sht) pht)) sht_lk;
-  with spht. assert (models sht_sig (dfst locked_sht) spht);
+  let sht_lk = locked_sht._2;
+  L.acquire #(exists_ (fun pht -> models sht_sig locked_sht._1 pht)) sht_lk;
+  with spht. assert (models sht_sig locked_sht._1 spht);
 
-  let res = HT.lookup #sht_sig #spht (dfst locked_sht) sid;
+  let res = HT.lookup #sht_sig #spht locked_sht._1 sid;
   if (fst res) {
     let opt_locked_cht = snd res;
     match opt_locked_cht {
     Some locked_cht -> {
-      let cht_lk = dsnd locked_cht;
-      L.acquire #(exists_ (fun pht -> models cht_sig (dfst locked_cht) pht)) cht_lk;
-      with cpht. assert (models cht_sig (dfst locked_cht) cpht);
-      let r = HT.lookup #cht_sig #cpht (dfst locked_cht) ctxt_hndl;
+      let cht_lk = locked_cht._2;
+      L.acquire #(exists_ (fun pht -> models cht_sig locked_cht._1 pht)) cht_lk;
+      with cpht. assert (models cht_sig locked_cht._1 cpht);
+      let r = HT.lookup #cht_sig #cpht locked_cht._1 ctxt_hndl;
       if (fst r) {
         let opt_locked_ctxt = snd r;
         match opt_locked_ctxt {
         Some locked_context -> {
-          let b = not_full #cht_sig #cpht (dfst locked_cht);
+          let b = not_full #cht_sig #cpht locked_cht._1;
           if b {
-            let r = HT.insert #cht_sig #cpht (dfst locked_cht) new_ctxt_hndl locked_context;
-            with cpht'. unfold (maybe_update r cht_sig (dfst locked_cht) cpht cpht'); // FIXME: why doesn't this work if we explicitly specify cpht and cpht'
+            let r = HT.insert #cht_sig #cpht locked_cht._1 new_ctxt_hndl locked_context;
+            with cpht'. unfold (maybe_update r cht_sig locked_cht._1 cpht cpht'); // FIXME: why doesn't this work if we explicitly specify cpht and cpht'
             if r {
-              assert (models cht_sig (dfst locked_cht) (PHT.insert cpht new_ctxt_hndl locked_context));
-              let d = HT.delete #cht_sig #(PHT.insert cpht new_ctxt_hndl locked_context) (dfst locked_cht) ctxt_hndl;
-              with x y. unfold (maybe_update d cht_sig (dfst locked_cht) x y); 
+              assert (models cht_sig locked_cht._1 (PHT.insert cpht new_ctxt_hndl locked_context));
+              let d = HT.delete #cht_sig #(PHT.insert cpht new_ctxt_hndl locked_context) locked_cht._1 ctxt_hndl;
+              with x y. unfold (maybe_update d cht_sig locked_cht._1 x y); 
               if d {
-                assert (models cht_sig (dfst locked_cht) (PHT.delete (PHT.insert cpht new_ctxt_hndl locked_context) ctxt_hndl));
-                L.release #(exists_ (fun pht -> models sht_sig (dfst locked_sht) pht)) sht_lk;
-                L.release #(exists_ (fun pht -> models cht_sig (dfst locked_cht) pht)) cht_lk;
+                assert (models cht_sig locked_cht._1 (PHT.delete (PHT.insert cpht new_ctxt_hndl locked_context) ctxt_hndl));
+                L.release #(exists_ (fun pht -> models sht_sig locked_sht._1 pht)) sht_lk;
+                L.release #(exists_ (fun pht -> models cht_sig locked_cht._1 pht)) cht_lk;
                 Some new_ctxt_hndl
               } else {
                 // ERROR - delete failed
-                assert (models cht_sig (dfst locked_cht) (PHT.insert cpht new_ctxt_hndl locked_context));
-                L.release #(exists_ (fun pht -> models sht_sig (dfst locked_sht) pht)) sht_lk;
-                L.release #(exists_ (fun pht -> models cht_sig (dfst locked_cht) pht)) cht_lk;
+                assert (models cht_sig locked_cht._1 (PHT.insert cpht new_ctxt_hndl locked_context));
+                L.release #(exists_ (fun pht -> models sht_sig locked_sht._1 pht)) sht_lk;
+                L.release #(exists_ (fun pht -> models cht_sig locked_cht._1 pht)) cht_lk;
                 None #ctxt_hndl_t
               }
             } else {
               // ERROR - insert failed
-              assert (models cht_sig (dfst locked_cht) cpht);
-              L.release #(exists_ (fun pht -> models sht_sig (dfst locked_sht) pht)) sht_lk;
-              L.release #(exists_ (fun pht -> models cht_sig (dfst locked_cht) pht)) cht_lk;  
+              assert (models cht_sig locked_cht._1 cpht);
+              L.release #(exists_ (fun pht -> models sht_sig locked_sht._1 pht)) sht_lk;
+              L.release #(exists_ (fun pht -> models cht_sig locked_cht._1 pht)) cht_lk;  
               None #ctxt_hndl_t
           }} else {
               // ERROR - table full
-              L.release #(exists_ (fun pht -> models sht_sig (dfst locked_sht) pht)) sht_lk;
-              L.release #(exists_ (fun pht -> models cht_sig (dfst locked_cht) pht)) cht_lk;
+              L.release #(exists_ (fun pht -> models sht_sig locked_sht._1 pht)) sht_lk;
+              L.release #(exists_ (fun pht -> models cht_sig locked_cht._1 pht)) cht_lk;
               None #ctxt_hndl_t
           }}
         None -> {
           // ERROR - bad context handle
-          L.release #(exists_ (fun pht -> models sht_sig (dfst locked_sht) pht)) sht_lk;
-          L.release #(exists_ (fun pht -> models cht_sig (dfst locked_cht) pht)) cht_lk;
+          L.release #(exists_ (fun pht -> models sht_sig locked_sht._1 pht)) sht_lk;
+          L.release #(exists_ (fun pht -> models cht_sig locked_cht._1 pht)) cht_lk;
           None #ctxt_hndl_t 
         }}
       } else {
         // ERROR - lookup failed
-        L.release #(exists_ (fun pht -> models sht_sig (dfst locked_sht) pht)) sht_lk;
-        L.release #(exists_ (fun pht -> models cht_sig (dfst locked_cht) pht)) cht_lk;
+        L.release #(exists_ (fun pht -> models sht_sig locked_sht._1 pht)) sht_lk;
+        L.release #(exists_ (fun pht -> models cht_sig locked_cht._1 pht)) cht_lk;
         None #ctxt_hndl_t 
       }}
     None -> {
       // ERROR - lookup context table failed
-      L.release #(exists_ (fun pht -> models sht_sig (dfst locked_sht) pht)) sht_lk;
+      L.release #(exists_ (fun pht -> models sht_sig locked_sht._1 pht)) sht_lk;
       None #ctxt_hndl_t 
     }}
   } else {
     // ERROR - lookup context table failed
-    L.release #(exists_ (fun pht -> models sht_sig (dfst locked_sht) pht)) sht_lk;
+    L.release #(exists_ (fun pht -> models sht_sig locked_sht._1 pht)) sht_lk;
     None #ctxt_hndl_t 
   }
 }
@@ -711,33 +844,34 @@ fn derive_child' (sid:sid_t) (ctxt_hndl:ctxt_hndl_t) (record:record_t) (#repr:er
 {
   let new_ctxt_hndl = prng ();
 
-  let sht_lk = dsnd locked_sht;
-  L.acquire #(exists_ (fun pht -> models sht_sig (dfst locked_sht) pht)) sht_lk;
-  with spht. assert (models sht_sig (dfst locked_sht) spht);
+  let sht_lk = locked_sht._2;
+  L.acquire #(exists_ (fun pht -> models sht_sig locked_sht._1 pht)) sht_lk;
+  with spht. assert (models sht_sig locked_sht._1 spht);
 
-  let res = HT.lookup #sht_sig #spht (dfst locked_sht) sid;
+  let res = HT.lookup #sht_sig #spht locked_sht._1 sid;
   if (fst res) {
     let opt_locked_cht = snd res;
     match opt_locked_cht {
     Some locked_cht -> {
-      let cht_lk = dsnd locked_cht;
-      L.acquire #(exists_ (fun pht -> models cht_sig (dfst locked_cht) pht)) cht_lk;
-      with cpht. assert (models cht_sig (dfst locked_cht) cpht);
+      let cht_lk = locked_cht._2;
+      L.acquire #(exists_ (fun pht -> models cht_sig locked_cht._1 pht)) cht_lk;
+      with cpht. assert (models cht_sig locked_cht._1 cpht);
 
-      let r = HT.lookup #cht_sig #cpht (dfst locked_cht) ctxt_hndl;
+      let r = HT.lookup #cht_sig #cpht locked_cht._1 ctxt_hndl;
       if (fst r) {
         let opt_locked_ctxt = snd r;
         match opt_locked_ctxt {
         Some locked_ctxt -> {
-        let ctxt = dfst locked_ctxt;
-        let ctxt_lk = dsnd locked_ctxt;
-        L.acquire #(context_perm ctxt) ctxt_lk;
+        let ctxt = locked_ctxt._1;
+        let ctxt_repr = locked_ctxt._2;
+        let ctxt_lk = locked_ctxt._3;
+        L.acquire #(context_perm ctxt ctxt_repr) ctxt_lk;
 
         match ctxt {
         Engine_context c -> {
           // NOTE: we won't eventually release engine_context_perm because we won't 
           // own it anymore -- we will disable the uds and free the uds array
-          rewrite (context_perm ctxt) as (engine_context_perm c);
+          rewrite (context_perm ctxt ctxt_repr) as (engine_context_perm c);
           unfold (engine_context_perm c);
 
           match record {
@@ -750,46 +884,46 @@ fn derive_child' (sid:sid_t) (ctxt_hndl:ctxt_hndl_t) (record:record_t) (#repr:er
             let ret = EngineCore.engine_main cdi c.uds r;
             with s. assert (A.pts_to cdi full_perm s);
             fold (engine_context_perm c);
-            rewrite (engine_context_perm c) as (context_perm ctxt);
+            rewrite (engine_context_perm c) as (context_perm ctxt ctxt_repr);
             destroy_ctxt ctxt;
 
             match ret {
             DICE_SUCCESS -> {
-              let new_locked_context = init_l0_ctxt cdi;
+              let new_locked_context = init_l0_ctxt cdi #r0 #s ();
               
-              let d = HT.delete #cht_sig #cpht (dfst locked_cht) ctxt_hndl;
-              with cpht'. unfold (maybe_update d cht_sig (dfst locked_cht) cpht cpht');
+              let d = HT.delete #cht_sig #cpht locked_cht._1 ctxt_hndl;
+              with cpht'. unfold (maybe_update d cht_sig locked_cht._1 cpht cpht');
               if d {
-                assert (models cht_sig (dfst locked_cht) (PHT.delete cpht ctxt_hndl));
-                let b = not_full #cht_sig #(PHT.delete cpht ctxt_hndl) (dfst locked_cht);
+                assert (models cht_sig locked_cht._1 (PHT.delete cpht ctxt_hndl));
+                let b = not_full #cht_sig #(PHT.delete cpht ctxt_hndl) locked_cht._1;
                 if b {
-                  let i = HT.insert #cht_sig #(PHT.delete cpht ctxt_hndl) (dfst locked_cht) new_ctxt_hndl new_locked_context; 
-                  with x y. unfold (maybe_update i cht_sig (dfst locked_cht) x y);
+                  let i = HT.insert #cht_sig #(PHT.delete cpht ctxt_hndl) locked_cht._1 new_ctxt_hndl new_locked_context; 
+                  with x y. unfold (maybe_update i cht_sig locked_cht._1 x y);
                   if i {
-                    assert (models cht_sig (dfst locked_cht) (PHT.insert (PHT.delete cpht ctxt_hndl) new_ctxt_hndl new_locked_context));
+                    assert (models cht_sig locked_cht._1 (PHT.insert (PHT.delete cpht ctxt_hndl) new_ctxt_hndl new_locked_context));
                     rewrite (engine_record_perm r r0) as (record_perm record repr);
-                    L.release #(exists_ (fun pht -> models sht_sig (dfst locked_sht) pht)) sht_lk;
-                    L.release #(exists_ (fun pht -> models cht_sig (dfst locked_cht) pht)) cht_lk;
+                    L.release #(exists_ (fun pht -> models sht_sig locked_sht._1 pht)) sht_lk;
+                    L.release #(exists_ (fun pht -> models cht_sig locked_cht._1 pht)) cht_lk;
                     Some new_ctxt_hndl
                   } else {
                     // ERROR - insert failed
-                    assert (models cht_sig (dfst locked_cht) (PHT.delete cpht ctxt_hndl));
+                    assert (models cht_sig locked_cht._1 (PHT.delete cpht ctxt_hndl));
                     rewrite (engine_record_perm r r0) as (record_perm record repr);
-                    L.release #(exists_ (fun pht -> models sht_sig (dfst locked_sht) pht)) sht_lk;
-                    L.release #(exists_ (fun pht -> models cht_sig (dfst locked_cht) pht)) cht_lk;
+                    L.release #(exists_ (fun pht -> models sht_sig locked_sht._1 pht)) sht_lk;
+                    L.release #(exists_ (fun pht -> models cht_sig locked_cht._1 pht)) cht_lk;
                     None #ctxt_hndl_t
                 }} else {
                   // ERROR - table full
                   rewrite (engine_record_perm r r0) as (record_perm record repr);
-                  L.release #(exists_ (fun pht -> models sht_sig (dfst locked_sht) pht)) sht_lk;
-                  L.release #(exists_ (fun pht -> models cht_sig (dfst locked_cht) pht)) cht_lk;
+                  L.release #(exists_ (fun pht -> models sht_sig locked_sht._1 pht)) sht_lk;
+                  L.release #(exists_ (fun pht -> models cht_sig locked_cht._1 pht)) cht_lk;
                   None #ctxt_hndl_t
               }} else {
                 // ERROR - delete failed
-                assert (models cht_sig (dfst locked_cht) cpht);
+                assert (models cht_sig locked_cht._1 cpht);
                 rewrite (engine_record_perm r r0) as (record_perm record repr);
-                L.release #(exists_ (fun pht -> models sht_sig (dfst locked_sht) pht)) sht_lk;
-                L.release #(exists_ (fun pht -> models cht_sig (dfst locked_cht) pht)) cht_lk;
+                L.release #(exists_ (fun pht -> models sht_sig locked_sht._1 pht)) sht_lk;
+                L.release #(exists_ (fun pht -> models cht_sig locked_cht._1 pht)) cht_lk;
                 None #ctxt_hndl_t
               }}
             DICE_ERROR -> {
@@ -797,26 +931,27 @@ fn derive_child' (sid:sid_t) (ctxt_hndl:ctxt_hndl_t) (record:record_t) (#repr:er
               A.zeroize dice_digest_len cdi;
               A.free cdi;
               rewrite (engine_record_perm r r0) as (record_perm record repr);
-              L.release #(exists_ (fun pht -> models sht_sig (dfst locked_sht) pht)) sht_lk;
-              L.release #(exists_ (fun pht -> models cht_sig (dfst locked_cht) pht)) cht_lk;
+              L.release #(exists_ (fun pht -> models sht_sig locked_sht._1 pht)) sht_lk;
+              L.release #(exists_ (fun pht -> models cht_sig locked_cht._1 pht)) cht_lk;
               None #ctxt_hndl_t
             }}}
           _ -> {
             // ERROR - record should have type (Engine_record r)
             fold (engine_context_perm c);
-            rewrite (engine_context_perm c) as (context_perm ctxt);
+            rewrite (engine_context_perm c) as (context_perm ctxt ctxt_repr);
             destroy_ctxt ctxt;
-            L.release #(exists_ (fun pht -> models sht_sig (dfst locked_sht) pht)) sht_lk;
-            L.release #(exists_ (fun pht -> models cht_sig (dfst locked_cht) pht)) cht_lk;
+            L.release #(exists_ (fun pht -> models sht_sig locked_sht._1 pht)) sht_lk;
+            L.release #(exists_ (fun pht -> models cht_sig locked_cht._1 pht)) cht_lk;
             None #ctxt_hndl_t
           }}
         }
         L0_context c -> {
           // NOTE: we won't eventually release l0_context_perm because we won't 
           // own it anymore -- we will free the cdi array
-          rewrite (context_perm ctxt) as (l0_context_perm c);
-          unfold (l0_context_perm c);
-
+          let cr = get_l0_context_perm ctxt ctxt_repr;
+          rewrite (l0_context_perm (L0_context?.c ctxt) cr)
+            as (l0_context_perm c cr);
+          unfold (l0_context_perm c cr);
           with s. assert (A.pts_to c.cdi full_perm s);
 
           match record {
@@ -848,15 +983,23 @@ fn derive_child' (sid:sid_t) (ctxt_hndl:ctxt_hndl_t) (record:record_t) (#repr:er
                             aliasKey_pub aliasKey_priv 
                             aliasKeyTBS_len aliasKeyCRT_len aliasKeyCRT 
                             deviceIDCRI_len deviceIDCSR_len deviceIDCSR r;
-            fold (l0_context_perm c);
-            rewrite (l0_context_perm c) as (context_perm ctxt);
+            fold (l0_context_perm c cr);
+            rewrite (l0_context_perm c cr) as (context_perm ctxt ctxt_repr);
             destroy_ctxt ctxt;
 
-            with (s1:elseq U8.t v32us). assert (A.pts_to aliasKey_priv full_perm s1);
-            let new_locked_context = init_l1_ctxt deviceIDCSR_len aliasKeyCRT_len 
-                                                  deviceID_priv deviceID_pub
-                                                  aliasKey_priv aliasKey_pub 
-                                                  deviceIDCSR aliasKeyCRT;
+            with deviceID_pub1. assert (A.pts_to deviceID_pub full_perm deviceID_pub1);
+            with deviceID_priv1. assert (A.pts_to deviceID_priv full_perm deviceID_priv1);
+            with aliasKey_pub1. assert (A.pts_to aliasKey_pub full_perm aliasKey_pub1);
+            with aliasKey_priv1. assert (A.pts_to aliasKey_priv full_perm aliasKey_priv1);
+            with deviceIDCSR1. assert (A.pts_to deviceIDCSR full_perm deviceIDCSR1);
+            with aliasKeyCRT1. assert (A.pts_to aliasKeyCRT full_perm aliasKeyCRT1);
+            let new_locked_context = init_l1_ctxt 
+              deviceIDCSR_len aliasKeyCRT_len deviceID_priv deviceID_pub
+              aliasKey_priv aliasKey_pub deviceIDCSR aliasKeyCRT
+              #deviceID_priv1 #deviceID_pub1 #aliasKey_priv1 #aliasKey_pub1
+              #deviceIDCSR1 #aliasKeyCRT1 #(hide r.deviceID_label_len)
+              #(hide r.aliasKey_label_len) #s #r0 #(hide idcsr_ing) #(hide akcrt_ing) ();
+            
             A.free deviceID_pub;
             A.free deviceID_priv;
             A.free aliasKey_pub;
@@ -864,78 +1007,78 @@ fn derive_child' (sid:sid_t) (ctxt_hndl:ctxt_hndl_t) (record:record_t) (#repr:er
             A.free deviceIDCSR;
             A.free aliasKeyCRT;
             
-            let d = HT.delete #cht_sig #cpht (dfst locked_cht) ctxt_hndl;
-            with x y. unfold (maybe_update d cht_sig (dfst locked_cht) x y);
+            let d = HT.delete #cht_sig #cpht locked_cht._1 ctxt_hndl;
+            with x y. unfold (maybe_update d cht_sig locked_cht._1 x y);
             if d {
-              assert (models cht_sig (dfst locked_cht) (PHT.delete cpht ctxt_hndl));
-              let b = not_full #cht_sig #(PHT.delete cpht ctxt_hndl) (dfst locked_cht);
+              assert (models cht_sig locked_cht._1 (PHT.delete cpht ctxt_hndl));
+              let b = not_full #cht_sig #(PHT.delete cpht ctxt_hndl) locked_cht._1;
               if b {
-                let i = HT.insert #cht_sig #(PHT.delete cpht ctxt_hndl) (dfst locked_cht) new_ctxt_hndl new_locked_context;
-                with x y. unfold (maybe_update i cht_sig (dfst locked_cht) x y);
+                let i = HT.insert #cht_sig #(PHT.delete cpht ctxt_hndl) locked_cht._1 new_ctxt_hndl new_locked_context;
+                with x y. unfold (maybe_update i cht_sig locked_cht._1 x y);
                 if i {
-                  assert (models cht_sig (dfst locked_cht) (PHT.insert (PHT.delete cpht ctxt_hndl) new_ctxt_hndl new_locked_context));
+                  assert (models cht_sig locked_cht._1 (PHT.insert (PHT.delete cpht ctxt_hndl) new_ctxt_hndl new_locked_context));
                   rewrite (l0_record_perm r r0) as (record_perm record repr);
-                  L.release #(exists_ (fun pht -> models sht_sig (dfst locked_sht) pht)) sht_lk;
-                  L.release #(exists_ (fun pht -> models cht_sig (dfst locked_cht) pht)) cht_lk;
+                  L.release #(exists_ (fun pht -> models sht_sig locked_sht._1 pht)) sht_lk;
+                  L.release #(exists_ (fun pht -> models cht_sig locked_cht._1 pht)) cht_lk;
                   Some new_ctxt_hndl
                 } else {
                   // ERROR - insert failed
-                  assert (models cht_sig (dfst locked_cht) (PHT.delete cpht ctxt_hndl));
+                  assert (models cht_sig locked_cht._1 (PHT.delete cpht ctxt_hndl));
                   rewrite (l0_record_perm r r0) as (record_perm record repr);
-                  L.release #(exists_ (fun pht -> models sht_sig (dfst locked_sht) pht)) sht_lk;
-                  L.release #(exists_ (fun pht -> models cht_sig (dfst locked_cht) pht)) cht_lk;
+                  L.release #(exists_ (fun pht -> models sht_sig locked_sht._1 pht)) sht_lk;
+                  L.release #(exists_ (fun pht -> models cht_sig locked_cht._1 pht)) cht_lk;
                   None #ctxt_hndl_t
               }} else {
                 // ERROR - table full
                 rewrite (l0_record_perm r r0) as (record_perm record repr);
-                L.release #(exists_ (fun pht -> models sht_sig (dfst locked_sht) pht)) sht_lk;
-                L.release #(exists_ (fun pht -> models cht_sig (dfst locked_cht) pht)) cht_lk;
+                L.release #(exists_ (fun pht -> models sht_sig locked_sht._1 pht)) sht_lk;
+                L.release #(exists_ (fun pht -> models cht_sig locked_cht._1 pht)) cht_lk;
                 None #ctxt_hndl_t
             }} else {
               // ERROR - delete failed
-              assert (models cht_sig (dfst locked_cht) cpht);
+              assert (models cht_sig locked_cht._1 cpht);
               rewrite (l0_record_perm r r0) as (record_perm record repr);
-              L.release #(exists_ (fun pht -> models sht_sig (dfst locked_sht) pht)) sht_lk;
-              L.release #(exists_ (fun pht -> models cht_sig (dfst locked_cht) pht)) cht_lk;
+              L.release #(exists_ (fun pht -> models sht_sig locked_sht._1 pht)) sht_lk;
+              L.release #(exists_ (fun pht -> models cht_sig locked_cht._1 pht)) cht_lk;
               None #ctxt_hndl_t
             }}
           _ -> {
             // ERROR - record should have type (L0_record r)
-            fold (l0_context_perm c);
-            rewrite (l0_context_perm c) as (context_perm ctxt);
+            fold (l0_context_perm c cr);
+            rewrite (l0_context_perm c cr) as (context_perm ctxt ctxt_repr);
             destroy_ctxt ctxt;
-            L.release #(exists_ (fun pht -> models sht_sig (dfst locked_sht) pht)) sht_lk;
-            L.release #(exists_ (fun pht -> models cht_sig (dfst locked_cht) pht)) cht_lk;
+            L.release #(exists_ (fun pht -> models sht_sig locked_sht._1 pht)) sht_lk;
+            L.release #(exists_ (fun pht -> models cht_sig locked_cht._1 pht)) cht_lk;
             None #ctxt_hndl_t
           }}
         }
         _ -> { 
           // ERROR - cannot invoke DeriveChild with L1 context
-          L.release #(context_perm ctxt) ctxt_lk;
-          L.release #(exists_ (fun pht -> models sht_sig (dfst locked_sht) pht)) sht_lk;
-          L.release #(exists_ (fun pht -> models cht_sig (dfst locked_cht) pht)) cht_lk;
+          L.release #(context_perm ctxt ctxt_repr) ctxt_lk;
+          L.release #(exists_ (fun pht -> models sht_sig locked_sht._1 pht)) sht_lk;
+          L.release #(exists_ (fun pht -> models cht_sig locked_cht._1 pht)) cht_lk;
           None #ctxt_hndl_t
         }}}
         None -> { 
         // ERROR - bad context handle
-        L.release #(exists_ (fun pht -> models sht_sig (dfst locked_sht) pht)) sht_lk;
-        L.release #(exists_ (fun pht -> models cht_sig (dfst locked_cht) pht)) cht_lk;
+        L.release #(exists_ (fun pht -> models sht_sig locked_sht._1 pht)) sht_lk;
+        L.release #(exists_ (fun pht -> models cht_sig locked_cht._1 pht)) cht_lk;
         None #ctxt_hndl_t
         }}
       } else {
         // ERROR - lookup failed
-        L.release #(exists_ (fun pht -> models sht_sig (dfst locked_sht) pht)) sht_lk;
-        L.release #(exists_ (fun pht -> models cht_sig (dfst locked_cht) pht)) cht_lk;
+        L.release #(exists_ (fun pht -> models sht_sig locked_sht._1 pht)) sht_lk;
+        L.release #(exists_ (fun pht -> models cht_sig locked_cht._1 pht)) cht_lk;
         None #ctxt_hndl_t
       }}
     None -> { 
     // ERROR - bad session ID
-    L.release #(exists_ (fun pht -> models sht_sig (dfst locked_sht) pht)) sht_lk;
+    L.release #(exists_ (fun pht -> models sht_sig locked_sht._1 pht)) sht_lk;
     None #ctxt_hndl_t
     }}
   } else {
     // ERROR - lookup failed
-    L.release #(exists_ (fun pht -> models sht_sig (dfst locked_sht) pht)) sht_lk;
+    L.release #(exists_ (fun pht -> models sht_sig locked_sht._1 pht)) sht_lk;
     None #ctxt_hndl_t
   }
 }
